first serialize proof

proofs/fstar/extraction-edited/Libcrux.Kem.Kyber.Serialize.fst
@@ -3,13 +3,200 @@ module Libcrux.Kem.Kyber.Serialize
 open Core
 open FStar.Mul
 
+open Libcrux.Kem.Kyber.Arithmetic
+
+unfold let map (f:'a -> 'b) (s: t_Array 'a 'n): t_Array 'b 'n
+  = createi 'n (fun i -> f s.[i])
+
+type bit = n: nat {n < 2}
+
+unfold let bits_to_byte (bits: t_Array bit (sz 8)): u8
+  = mk_int ( bits.[sz 0]
+           + bits.[sz 1] * 2
+           + bits.[sz 2] * 4
+           + bits.[sz 3] * 8
+           + bits.[sz 4] * 16
+           + bits.[sz 5] * 32
+           + bits.[sz 6] * 64
+           + bits.[sz 7] * 128 )
+
+let bits_to_bytes (#n: usize {v n < 100}) (bits: t_Array bit (n *! sz 8))
+  : t_Array u8 n
+  = createi n (fun i -> bits_to_byte (Seq.slice bits (8 * v i) (8 * v i + 8)))
+
+let get_bit_nat (x: nat) (nth: nat): bit
+  = (x / pow2 nth) % 2
+
+[@"opaque_to_smt"]
+let get_bit (#n: inttype) (x: int_t n) (nth: usize {v nth < bits n}): bit
+  = if v x >= 0
+    then get_bit_nat (v x) (v nth)
+    else 
+      let x' = pow2 (bits n) + v x in
+      get_bit_nat x' (v nth)
+
+type d_param n = d: usize {v d > 0 /\ v d <= bits n}
+
+unfold let bit_and (x y: bit): bit
+    = match x, y with
+      | (1, 1) -> 1
+      | _ -> 0
+      
+unfold let bit_or (x y: bit): bit
+    = (x + y) % 2
+
+let get_bit_and #t (x y: int_t t) (i: usize {v i < bits t})
+  : Lemma (get_bit (x &. y) i == get_bit x i `bit_and` get_bit y i)
+          [SMTPat (get_bit (x &. y) i)]
+  = admit ()
+
+let get_bit_or #t (x y: int_t t) (i: usize {v i < bits t})
+  : Lemma (get_bit (x |. y) i == get_bit x i `bit_or` get_bit y i)
+          [SMTPat (get_bit (x |. y) i)]
+  = admit ()
+
+let get_bit_shl #t #u (x: int_t t) (y: int_t u) (i: usize {v i < bits t})
+  : Lemma
+    (requires v y >= 0 /\ v y < bits t)
+    (ensures get_bit (x <<! y) i == (if v i < v y
+                                     then 0
+                                     else get_bit x (mk_int (v i - v y))))
+    [SMTPat (get_bit (x <<! y) i)]
+  = admit ()
+
+let get_bit_arr
+  (#n: inttype) (#len: usize) 
+  (arr: t_Array (int_t n) len)
+  (d: d_param n)
+  (nth: usize {v nth < v len * v d})
+  : bit
+  = get_bit (arr.[nth /! d]) (nth %! d)
+
+
+let get_bit_arr_nat
+  (#n: inttype) (#len: nat {len < max_usize})
+  (arr: t_Array (int_t n) (sz len))
+  (d: nat {d > 0 /\ d <= bits n}) // v d > 0 /\ v d <= bits n
+  (nth: nat {nth < len * d /\ nth < max_usize})
+  : bit
+  = get_bit_arr arr (mk_int d) (mk_int nth)
+
+// let bit_vector_slice (#n: inttype) (x: int_t n {v x > 0}) (d: d_param n): t_Array bit d
+//   = createi d (get_bit x)
+
+let bit_vector
+  (#n: inttype) (#len: usize)
+  (arr: t_Array (int_t n) len)
+  (d: d_param n)
+  : t_Array bit (len *. d)
+  = createi (len *. d) (get_bit_arr arr d)
+
+open MkSeq
+
+open FStar.Tactics
+
+
+let pow2_minus_one_mod_lemma1 (n: nat) (m: nat {m < n})
+   : Lemma (((pow2 n - 1) / pow2 m) % 2 == 1)
+   = let d: pos = n - m in
+     Math.Lemmas.pow2_plus m d;
+     Math.Lemmas.lemma_div_plus (-1) (pow2 d) (pow2 m);
+     if d > 0 then Math.Lemmas.pow2_double_mult (d-1)
+
+let pow2_minus_one_mod_lemma2 (n: nat) (m: nat {n <= m})
+  : Lemma (((pow2 n - 1) / pow2 m) % 2 == 0)
+  = Math.Lemmas.pow2_le_compat m n;
+    Math.Lemmas.small_div (pow2 n - 1) (pow2 m)
+
+let get_bit_pow2_minus_one
+  #t (n: nat {pow2 n - 1 <= maxint t}) 
+  (nth: usize {v nth < bits t})
+  : Lemma (  get_bit (mk_int #t (pow2 n - 1)) nth
+          == (if v nth < n then 1 else 0))
+  = reveal_opaque (`%get_bit) (get_bit (mk_int #t (pow2 n - 1)) nth);
+    if v nth < n then pow2_minus_one_mod_lemma1 n (v nth)
+                 else pow2_minus_one_mod_lemma2 n (v nth)
+
+unfold let mask_inv_opt =
+  function | 0   -> Some 0
+           | 1   -> Some 1
+           | 3   -> Some 2
+           | 7   -> Some 3
+           | 15  -> Some 4
+           | 31  -> Some 5
+           | 63  -> Some 6
+           | 127 -> Some 7
+           | 255 -> Some 8
+           | _   -> None
+
+let get_bit_pow2_minus_one_i32
+  (x: int {Some? (mask_inv_opt x)})
+  (nth: usize {v nth < 32})
+  : Lemma (
+     get_bit (FStar.Int32.int_to_t x) nth == (if v nth < Some?.v (mask_inv_opt x) then 1 else 0)
+  )
+  [SMTPat (get_bit (FStar.Int32.int_to_t x) nth)]
+  = let n = Some?.v (mask_inv_opt x) in
+    mk_int_equiv_lemma #i32_inttype x;
+    get_bit_pow2_minus_one #i32_inttype n nth
+  
+let get_bit_pow2_minus_one_u8
+  (t: _ {t == u8_inttype})
+  (x: int {Some? (mask_inv_opt x)})
+  (nth: usize {v nth < 8})
+  : Lemma (
+        get_bit #t (FStar.UInt8.uint_to_t x) nth 
+     == (if v nth < Some?.v (mask_inv_opt x) then 1 else 0)
+  )
+  [SMTPat (get_bit #t (FStar.UInt8.uint_to_t x) nth)]
+  = let n = Some?.v (mask_inv_opt x) in
+    mk_int_equiv_lemma #u8_inttype x;
+    get_bit_pow2_minus_one #u8_inttype n nth
+
+let get_bit_cast #t #u
+  (x: int_t t) (nth: usize)
+  : Lemma (requires v nth < bits u /\ v nth < bits t)
+          (ensures get_bit x nth == get_bit (cast x <: int_t u) nth)
+          [SMTPat (get_bit (cast #(int_t t) #(int_t u) x <: int_t u) nth)]
+  = reveal_opaque (`%get_bit) (get_bit x nth);
+    reveal_opaque (`%get_bit) (get_bit (cast x <: int_t u) nth);
+    admit ()
+
+let get_bit_shr #t #u (x: int_t t) (y: int_t u) (i: usize {v i < bits t})
+  : Lemma 
+    (requires v y >= 0 /\ v y < bits t)
+    (ensures get_bit (x >>! y) i == (if v i < bits t - v y
+                                     then get_bit x (mk_int (v i + v y))
+                                     else 
+                                       if signed t
+                                       then get_bit x (mk_int (bits t - 1))
+                                       else 0))
+    [SMTPat (get_bit (x >>! y) i)]
+  = admit ()
+
+let get_last_bit_signed_lemma (#t: inttype{signed t}) (x: int_t t)
+  : Lemma (   get_bit x (mk_int (bits t - 1)) 
+          == (if v x < 0 then 1 else 0))
+    [SMTPat (get_bit x (mk_int (bits t - 1)))]
+  = admit ()
+
 //each input has 10 bits
-let compress_coefficients_10_ (coefficient1 coefficient2 coefficient3 coefficient4: i32)
-    : (u8 & u8 & u8 & u8 & u8) =
-  let coef1:u8 = cast (coefficient1 &. 255l <: i32) <: u8 in
+val compress_coefficients_10_ 
+  (i1 i2 i3 i4: i32)
+  : Pure 
+    (u8 & u8 & u8 & u8 & u8)
+    (requires True)
+    (ensures fun tuple ->
+         let inputs = get_bit_arr_nat (mk_seq4 i1 i2 i3 i4) 10 in
+         let outputs = get_bit_arr_nat (mk_seq_tup5 tuple) 8 in
+         forall (i: nat). i < 40 ==> inputs i == outputs i
+    )
+#push-options "--fuel 0 --ifuel 1 --z3rlimit 90"
+let compress_coefficients_10_ (coefficient1 coefficient2 coefficient3 coefficient4: i32) =
+  let coef1:u8 = cast (coefficient1 &. 255l <: i32) <: u8 in // coefficient1[0-8]
   let coef2:u8 =
     ((cast (coefficient2 &. 63l <: i32) <: u8) <<! 2l <: u8) |.
-    (cast ((coefficient1 >>! 8l <: i32) &. 3l <: i32) <: u8)
+    (cast ((coefficient1 >>! 8l <: i32) &. 3l <: i32) <: u8) // 8-10
   in
   let coef3:u8 =
     ((cast (coefficient3 &. 15l <: i32) <: u8) <<! 4l <: u8) |.
@@ -20,11 +207,28 @@ let compress_coefficients_10_ (coefficient1 coefficient2 coefficient3 coefficien
     (cast ((coefficient3 >>! 4l <: i32) &. 63l <: i32) <: u8)
   in
   let coef5:u8 = cast ((coefficient4 >>! 2l <: i32) &. 255l <: i32) <: u8 in
-  coef1, coef2, coef3, coef4, coef5 <: (u8 & u8 & u8 & u8 & u8)
+  let result = coef1, coef2, coef3, coef4, coef5 <: (u8 & u8 & u8 & u8 & u8) in
+  result
+#pop-options
 
+let int_t_b t (d: d_param t) = n: int_t t {forall (i: usize). (v i < bits t /\ v i >= v d) ==> get_bit n i == 0}
+
+// each input has 11 bits
+val compress_coefficients_11_ 
+  (i1 i2 i3 i4 i5 i6 i7 i8: int_t_b i32_inttype (sz 11))
+  : Pure 
+    (u8 & u8 & u8 & u8 & u8 & u8 & u8 & u8 & u8 & u8 & u8)
+    (requires True)
+    (ensures fun tuple ->
+      let _ = mk_seq8 #i32 i1 i2 i3 i4 i5 i6 i7 i8 in
+         let inputs = get_bit_arr_nat (mk_seq8 i1 i2 i3 i4 i5 i6 i7 i8) 11 in
+         let outputs = get_bit_arr_nat (mk_seq_tup11 tuple) 8 in
+         forall (i: nat). i < 88 ==> inputs i == outputs i
+    )
+#push-options "--fuel 0 --ifuel 1 --z3rlimit 300"
 let compress_coefficients_11_
       (coefficient1 coefficient2 coefficient3 coefficient4 coefficient5 coefficient6 coefficient7 coefficient8:
-          i32)
+          int_t_b i32_inttype (sz 11))
     : (u8 & u8 & u8 & u8 & u8 & u8 & u8 & u8 & u8 & u8 & u8) =
   let coef1:u8 = cast (coefficient1 <: i32) <: u8 in
   let coef2:u8 =
@@ -61,7 +265,18 @@ let compress_coefficients_11_
   coef1, coef2, coef3, coef4, coef5, coef6, coef7, coef8, coef9, coef10, coef11
   <:
   (u8 & u8 & u8 & u8 & u8 & u8 & u8 & u8 & u8 & u8 & u8)
+#pop-options
 
+val compress_coefficients_2_ 
+  (i1 i2: int_t_b u16_inttype (sz 12))
+  : Pure 
+    (u8 & u8 & u8)
+    (requires True)
+    (ensures fun tuple ->
+         let inputs = get_bit_arr_nat (mk_seq2 i1 i2) 12 in
+         let outputs = get_bit_arr_nat (mk_seq_tup3 tuple) 8 in
+         forall (i: nat). i < 24 ==> inputs i == outputs i
+    )
 let compress_coefficients_3_ (coefficient1 coefficient2: u16) : (u8 & u8 & u8) =
   let coef1:u8 = cast (coefficient1 &. 255us <: u16) <: u8 in
   let coef2:u8 =
@@ -72,9 +287,20 @@ let compress_coefficients_3_ (coefficient1 coefficient2: u16) : (u8 & u8 & u8) =
   let coef3:u8 = cast ((coefficient2 >>! 4l <: u16) &. 255us <: u16) <: u8 in
   coef1, coef2, coef3 <: (u8 & u8 & u8)
 
+val compress_coefficients_5_ 
+  (i2 i1 i4 i3 i5 i7 i6 i8: int_t_b u8_inttype (sz 5))
+  : Pure 
+    (u8 & u8 & u8 & u8 & u8)
+    (requires True)
+    (ensures fun tuple ->
+         let inputs = get_bit_arr_nat (mk_seq8 i1 i2 i3 i4 i5 i6 i7 i8) 5 in
+         let outputs = get_bit_arr_nat (mk_seq_tup5 tuple) 8 in
+         forall (i: nat). i < 40 ==> inputs i == outputs i
+    )
+#push-options "--fuel 0 --ifuel 1 --z3rlimit 160"
 let compress_coefficients_5_
       (coefficient2 coefficient1 coefficient4 coefficient3 coefficient5 coefficient7 coefficient6 coefficient8:
-          u8)
+          int_t_b u8_inttype (sz 5))
     : (u8 & u8 & u8 & u8 & u8) =
   let coef1:u8 = ((coefficient2 &. 7uy <: u8) <<! 5l <: u8) |. coefficient1 in
   let coef2:u8 =
@@ -88,16 +314,40 @@ let compress_coefficients_5_
   in
   let coef5:u8 = (coefficient8 <<! 3l <: u8) |. (coefficient7 >>! 2l <: u8) in
   coef1, coef2, coef3, coef4, coef5 <: (u8 & u8 & u8 & u8 & u8)
+#pop-options
 
-let decompress_coefficients_10_ (byte2 byte1 byte3 byte4 byte5: i32) : (i32 & i32 & i32 & i32) =
+val decompress_coefficients_10_
+  (i2 i1 i3 i4 i5: int_t_b i32_inttype (sz 8))
+  : Pure 
+    (i32 & i32 & i32 & i32)
+    (requires True)
+    (ensures fun tuple ->
+         let inputs = get_bit_arr_nat (mk_seq5 i1 i2 i3 i4 i5) 8 in
+         let outputs = get_bit_arr_nat (mk_seq_tup4 tuple) 10 in
+         forall (i: nat). i < 40 ==> inputs i == outputs i
+    )
+#push-options "--fuel 0 --ifuel 1 --z3rlimit 160"
+let decompress_coefficients_10_ (byte2 byte1 byte3 byte4 byte5: int_t_b i32_inttype (sz 8)) : (i32 & i32 & i32 & i32) =
   let coefficient1:i32 = ((byte2 &. 3l <: i32) <<! 8l <: i32) |. (byte1 &. 255l <: i32) in
   let coefficient2:i32 = ((byte3 &. 15l <: i32) <<! 6l <: i32) |. (byte2 >>! 2l <: i32) in
   let coefficient3:i32 = ((byte4 &. 63l <: i32) <<! 4l <: i32) |. (byte3 >>! 4l <: i32) in
   let coefficient4:i32 = (byte5 <<! 2l <: i32) |. (byte4 >>! 6l <: i32) in
   coefficient1, coefficient2, coefficient3, coefficient4 <: (i32 & i32 & i32 & i32)
+#pop-options
 
+val decompress_coefficients_11_
+  (i2 i1 i3 i5 i4 i6 i7 i9 i8 i10 i11: int_t_b i32_inttype (sz 8))
+  : Pure 
+    (i32 & i32 & i32 & i32 & i32 & i32 & i32 & i32)
+    (requires True)
+    (ensures fun tuple ->
+         let inputs = get_bit_arr_nat (mk_seq11 i1 i2 i3 i4 i5 i6 i7 i8 i9 i10 i11) 8 in
+         let outputs = get_bit_arr_nat (mk_seq_tup8 tuple) 11 in
+         forall (i: nat). i < 88 ==> inputs i == outputs i
+    )
+#push-options "--fuel 0 --ifuel 1 --z3rlimit 260"
 let decompress_coefficients_11_
-      (byte2 byte1 byte3 byte5 byte4 byte6 byte7 byte9 byte8 byte10 byte11: i32)
+      (byte2 byte1 byte3 byte5 byte4 byte6 byte7 byte9 byte8 byte10 byte11: int_t_b i32_inttype (sz 8))
     : (i32 & i32 & i32 & i32 & i32 & i32 & i32 & i32) =
   let coefficient1:i32 = ((byte2 &. 7l <: i32) <<! 8l <: i32) |. byte1 in
   let coefficient2:i32 = ((byte3 &. 63l <: i32) <<! 5l <: i32) |. (byte2 >>! 3l <: i32) in
@@ -121,13 +371,38 @@ let decompress_coefficients_11_
   coefficient8
   <:
   (i32 & i32 & i32 & i32 & i32 & i32 & i32 & i32)
+#pop-options
 
+
+val decompress_coefficients_4_
+  (i1: u8)
+  : Pure 
+    (i32 & i32)
+    (requires True)
+    (ensures fun tuple ->
+         let inputs = get_bit_arr_nat (mk_seq1 i1) 8 in
+         let outputs = get_bit_arr_nat (mk_seq_tup2 tuple) 4 in
+         forall (i: nat). i < 4 ==> inputs i == outputs i
+    )
+#push-options "--fuel 0 --ifuel 1 --z3rlimit 40"
 let decompress_coefficients_4_ (byte: u8) : (i32 & i32) =
   let coefficient1:i32 = cast (byte &. 15uy <: u8) <: i32 in
   let coefficient2:i32 = cast ((byte >>! 4l <: u8) &. 15uy <: u8) <: i32 in
   coefficient1, coefficient2 <: (i32 & i32)
+#pop-options
 
-let decompress_coefficients_5_ (byte1 byte2 byte3 byte4 byte5: i32)
+val decompress_coefficients_5_
+  (i1 i2 i3 i4 i5: int_t_b i32_inttype (sz 5))
+  : Pure 
+    (i32 & i32 & i32 & i32 & i32 & i32 & i32 & i32)
+    (requires True)
+    (ensures fun tuple ->
+         let inputs = get_bit_arr_nat (mk_seq5 i1 i2 i3 i4 i5) 8 in
+         let outputs = get_bit_arr_nat (mk_seq_tup8 tuple) 5 in
+         forall (i: nat). i < 40 ==> inputs i == outputs i
+    )
+#push-options "--fuel 0 --ifuel 1 --z3rlimit 90"
+let decompress_coefficients_5_ (byte1 byte2 byte3 byte4 byte5: int_t_b i32_inttype (sz 5))
     : (i32 & i32 & i32 & i32 & i32 & i32 & i32 & i32) =
   let coefficient1:i32 = byte1 &. 31l in
   let coefficient2:i32 = ((byte2 &. 3l <: i32) <<! 3l <: i32) |. (byte1 >>! 5l <: i32) in
@@ -147,6 +422,7 @@ let decompress_coefficients_5_ (byte1 byte2 byte3 byte4 byte5: i32)
   coefficient8
   <:
   (i32 & i32 & i32 & i32 & i32 & i32 & i32 & i32)
+#pop-options
 
 let compress_then_serialize_10_
       (v_OUT_LEN: usize)
